llvm2acl2/acl2/cbrt-step-jvmN.lisp
@@ -34,6 +34,18 @@
                   val))
   :enable (load-i32 store-i32))
 
+(defrule load-i32-diff-store-i32
+  (implies (not (equal (car adr1) (car adr2)))
+           (equal (load-i32 adr1 (store-i32 val adr2 mem))
+                  (load-i32 adr1 mem)))
+  :enable (load-i32 store-i32))
+
+(defrule load-i32-diff-store-double
+  (implies (not (equal (car adr1) (car adr2)))
+           (equal (load-i32 adr1 (store-double val adr2 mem))
+                  (load-i32 adr1 mem)))
+  :enable (load-i32 store-double))
+
 (defrule load-i32-lv-0
   (implies (doublep (load-double (cons lv 0) mem))
            (equal (load-i32 (cons lv 0) mem)
@@ -60,6 +72,38 @@
                   (set-hi (load-double (cons lv 0) mem) i)))
   :enable (set-hi load-double store-i32)
   :expand (update-nth 1 (get-lo-i32 i) (cdr (assoc-equal lv mem))))
+
+(defruled logand-thm
+  (implies (and (i32p x)
+                (i32p y))
+           (equal (logand x y)
+                  (and-i32 x y)))
+  :enable and-i32
+  :disable logand)
+
+(defruled logior-thm
+  (implies (and (i32p x)
+                (i32p y))
+           (equal (logior x y)
+                  (or-i32 x y)))
+  :enable or-i32
+  :disable logior)
+
+(defruled logxor-thm
+  (implies (and (i32p x)
+                (i32p y))
+           (equal (logxor x y)
+                  (xor-i32 x y)))
+  :enable xor-i32
+  :disable logxor)
+
+(defruled fpadd-thm
+  (implies (and (doublep x)
+                (doublep y))
+           (equal (m5::fpadd x y (rtl::dp))
+                  (fadd-double x y)))
+  :enable fadd-double
+  :disable m5::fpadd)
 
 ;----------------------
 
@@ -176,7 +220,7 @@
 (defund cbrt-compute-program-p (program)
   (equal program *cbrt-compute-program*))
 
-(defrule index-into-cbrt-compute-progam
+(defrule index-into-cbrt-compute-program
   (implies (cbrt-compute-program-p program)
            (equal (m5::index-into-program byte-offset program)
                   (m5::index-into-program byte-offset *cbrt-compute-program*)))
@@ -239,7 +283,8 @@
   (implies (and (class-table-assumptions (m5::class-table s))
                 (equal (m5::status th s) 'm5::scheduled)
                 (member (m5::pc (m5::top-frame th s)) '(31))
-                (equal (m5::program (m5::top-frame th s)) *cbrt-compute-program*)
+                (cbrt-compute-program-p (m5::program (m5::top-frame th s)))
+;                (equal (m5::program (m5::top-frame th s)) *cbrt-compute-program*)
                 (equal (m5::cur-class (m5::top-frame th s)) "FdlibmTranslitN$Cbrt")
                 (doublep (m5::top (m5::pop (m5::stack (m5::top-frame th s))))))
            (poised-to-invoke-get-lo-p th s))
@@ -262,7 +307,8 @@
   (implies (and (class-table-assumptions (m5::class-table s))
                 (equal (m5::status th s) 'm5::scheduled)
                 (member (m5::pc (m5::top-frame th s)) '(147))
-                (equal (m5::program (m5::top-frame th s)) *cbrt-compute-program*)
+                (cbrt-compute-program-p (m5::program (m5::top-frame th s)))
+;                (equal (m5::program (m5::top-frame th s)) *cbrt-compute-program*)
                 (equal (m5::cur-class (m5::top-frame th s)) "FdlibmTranslitN$Cbrt")
                 (doublep (m5::top (m5::pop (m5::pop (m5::stack (m5::top-frame th s))))))
                 (i32p (m5::top (m5::stack (m5::top-frame th s)))))
@@ -274,13 +320,19 @@
   (implies (and (class-table-assumptions (m5::class-table s))
                 (equal (m5::status th s) 'm5::scheduled)
                 (member (m5::pc (m5::top-frame th s)) '(42 56 79 95 161 214))
-                (equal (m5::program (m5::top-frame th s)) *cbrt-compute-program*)
+                (cbrt-compute-program-p (m5::program (m5::top-frame th s)))
+;                (equal (m5::program (m5::top-frame th s)) *cbrt-compute-program*)
                 (equal (m5::cur-class (m5::top-frame th s)) "FdlibmTranslitN$Cbrt")
                 (doublep (m5::top (m5::pop (m5::pop (m5::stack (m5::top-frame th s))))))
                 (i32p (m5::top (m5::stack (m5::top-frame th s)))))
            (poised-to-invoke-set-hi-p th s))
   :enable poised-to-invoke-set-hi-p
   :disable m5::bound?)
+
+(defund ret-double (th s d)
+  (m5::modify
+   th s
+   :stack (m5::push2 d (m5::stack (m5::top-frame th s)))))
 
 ;-----------------------
 
@@ -383,6 +435,13 @@
        (pair-double-p mem 'w locals 9)
        (pair-i32-p mem 'sign locals 11)))
 
+(defrule pair-store-double-ret
+  (implies
+   (pair-p mem locals)
+   (pair-p (store-double d '(ret . 0) mem)
+           locals))
+  :enable (pair-p pair-double-p pair-i32-p))
+
 (defrule pair-x
   (implies (and (pair-p mem locals)
                 (doublep (load-double '(x . 0) mem)))
@@ -390,7 +449,7 @@
                   (load-double '(x . 0) mem)))
   :enable pair-p
   :use (:instance pair-double-thm (lv 'x) (jv 0)))
-           
+
 (defrule pair-store-double-x
   (implies
    (pair-p mem locals)
@@ -408,7 +467,7 @@
                   (load-i32 '(hx . 0) mem)))
   :enable pair-p
   :use (:instance pair-i32-thm (lv 'hx) (jv 2)))
-           
+
 (defrule pair-store-i32-hx
   (implies
    (pair-p mem locals)
@@ -425,7 +484,7 @@
                   (load-double '(r . 0) mem)))
   :enable pair-p
   :use (:instance pair-double-thm (lv 'r) (jv 3)))
-           
+
 (defrule pair-store-double-r
   (implies
    (pair-p mem locals)
@@ -443,7 +502,7 @@
                   (load-double '(s . 0) mem)))
   :enable pair-p
   :use (:instance pair-double-thm (lv 's) (jv 5)))
-           
+
 (defrule pair-store-double-s
   (implies
    (pair-p mem locals)
@@ -461,7 +520,7 @@
                   (load-double '(t . 0) mem)))
   :enable pair-p
   :use (:instance pair-double-thm (lv 't) (jv 7)))
-           
+
 (defrule pair-store-double-t
   (implies
    (pair-p mem locals)
@@ -476,7 +535,7 @@
                   (load-double '(w . 0) mem)))
   :enable pair-p
   :use (:instance pair-double-thm (lv 'w) (jv 9)))
-           
+
 (defrule pair-store-double-w
   (implies
    (pair-p mem locals)
@@ -494,7 +553,7 @@
                   (load-i32 '(sign . 0) mem)))
   :enable pair-p
   :use (:instance pair-i32-thm (lv 'sign) (jv 11)))
-                    
+
 (defrule pair-store-i32-sign
   (implies
    (pair-p mem locals)
@@ -522,84 +581,58 @@
      :status 'jvm::scheduled
      :call-stack (m5::push frame (m5::call-stack th sb)))))
 
-(defrule class-table-of-initial-s
-  (equal (m5::class-table (initial-s sb th x))
-         (m5::class-table sb))
-  :enable initial-s)
+(defund alpha (mem loc sb th s pc)
+  (let ((frame (m5::top-frame th s)))
+    (and (@cbrt-local-vars-p loc)
+         (@cbrt-mem-p mem)
+         (pair-p mem (m5::locals frame))
+         (class-table-assumptions (m5::class-table s))
+         (equal (m5::status th s) 'm5::scheduled)
+         (equal (m5::modify th s :call-stack (m5::pop (m5::call-stack th s))) sb)
+         (equal (m5::pc frame) pc)
+         (cbrt-compute-program-p (m5::program frame))
+         (equal (m5::sync-flg frame) 'jvm::unlocked)
+         (equal (m5::cur-class frame) "FdlibmTranslitN$Cbrt"))))
 
-(defrule status-of-initial-s
-  (equal (m5::status th (initial-s sb th x))
-         'jvm::scheduled)
-  :enable initial-s)
+(defrule class-table-of-sb-when-alpha
+  (implies (alpha mem loc sb th s pc)
+           (equal (m5::class-table s)
+                  (m5::class-table sb)))
+  :enable alpha)
 
-(defrule pc-of-initial-s
-  (equal (m5::pc (m5::top-frame th (initial-s sb th x)))
-         0)
-  :enable initial-s)
+(defrule status-of-sb-when-alpha
+  (implies (alpha mem loc sb th s pc)
+           (equal (m5::status th s)
+                  (m5::status th sb)))
+  :enable alpha)
 
-(defrule pc-of-initial-s_1
-  (equal (m5::pc (m5::top (m5::call-stack th (initial-s sb th x))))
-         0)
-  :enable initial-s)
+(defruled ret-thm-when-alpha
+  (implies
+   (and (alpha mem loc sb th s pc)
+        (member pc '(28 39 221)))
+   (equal
+    (m5::step th s)
+    (ret-double th sb (m5::top2 (m5::stack (m5::top-frame th s))))))
+  :enable (alpha ret-double)
+  :disable m5::bound?)
 
-(defrule locals-of-initial-s
-  (equal (m5::locals (m5::top-frame th (initial-s sb th x)))
-         (list x nil))
-  :enable initial-s)
-
-(defrule stack-of-initial-s
-  (equal (m5::stack (m5::top-frame th (initial-s sb th x)))
-         ())
-  :enable initial-s)
-
-(defrule program-of-initial-s
-  (cbrt-compute-program-p (m5::program (m5::top-frame th (initial-s sb th s))))
-  :enable initial-s)
-
-(defrule program-of-initial-s_1
-  (cbrt-compute-program-p (m5::program (m5::top (m5::call-stack th (initial-s sb th s)))))
-  :enable initial-s)
-
-(defrule sync-flg-of-initial-s
-  (equal (m5::sync-flg (m5::top-frame th (initial-s sb th x)))
-         'm5::unlocked)
-  :enable initial-s)
-
-(defrule cur-class-of-initial-s
-  (equal (m5::cur-class (m5::top-frame th (initial-s sb th x)))
-         "FdlibmTranslitN$Cbrt")
-  :enable initial-s)
+(defrule g-1-when-alpha
+  (implies (alpha mem loc sb th s pc)
+           (equal (g '%1 loc) '(ret . 0)))
+  :enable alpha)
 
 (defruled ttt-%0-m0.1
   (b* (
     (loc (@cbrt-%sign-loc (initial-s0 x)))
     (mem (@cbrt-m0.1-mem (initial-s0 x)))
     (s (initial-s sb th x))
-    (frame (m5::top-frame th s)))
+    (fixed-sb (m5::modify th sb :call-stack (m5::call-stack th sb) :status 'm5::scheduled)))
     (implies
      (and (doublep x)
           (class-table-assumptions (m5::class-table sb)))
-     (and (@cbrt-local-vars-p loc)
-          (@cbrt-mem-p mem)
-          (pair-p mem (m5::locals frame))
-          (class-table-assumptions (m5::class-table s))
-          (equal (m5::status th s) 'm5::scheduled)
-          (equal (m5::pc frame) 0)
-          (cbrt-compute-program-p (m5::program frame))
-          (equal (m5::cur-class frame) "FdlibmTranslitN$Cbrt")
-          (doublep (load-double '(x . 0) mem))
-;          (equal (nth 0 (m5::locals frame)) (load-double '(x . 0)))
-;          (equal mem
-;                 `((ret nil nil)
-;                   (x ,(get-lo-double x) ,(get-hi-double x))
-;                   (hx nil)
-;                   (r nil nil)
-;                   (s nil nil)
-;                   (t nil nil)
-;                   (w nil nil)
-;                   (sign nil)))
-          )))
-  :enable (initial-s0 pair-p
+     (and (alpha mem loc fixed-sb th s 0)
+          (doublep (load-double '(x . 0) mem)))))
+  :enable (alpha initial-s0 initial-s pair-p
            pair-double-p store-double load-double
            pair-i32-p load-i32
            @cbrt-local-vars-p
@@ -622,8 +655,7 @@
            @cbrt-%w-loc
            @cbrt-%sign-mem
            @cbrt-%sign-loc
-           @cbrt-m0.1-mem)
-  :disable m5::top-frame)
+           @cbrt-m0.1-mem))
 
 (defund sched-m0.2 (th)
   (m5::repeat th 2))
@@ -633,21 +665,14 @@
     (loc (@cbrt-%sign-loc (initial-s0 x)))
     (mem (@cbrt-m0.2-mem (initial-s0 x)))
     (s (m5::run (sched-m0.2 th) (initial-s sb th x)))
-    (frame (m5::top-frame th s)))
+    (fixed-sb (m5::modify th sb :call-stack (m5::call-stack th sb) :status 'm5::scheduled)))
     (implies
      (and (doublep x)
           (class-table-assumptions (m5::class-table sb)))
-     (and (@cbrt-local-vars-p loc)
-          (@cbrt-mem-p mem)
-          (pair-p mem (m5::locals frame))
-          (class-table-assumptions (m5::class-table s))
-          (equal (m5::status th s) 'm5::scheduled)
-          (equal (m5::pc frame) 3)
-          (cbrt-compute-program-p (m5::program frame))
-          (equal (m5::cur-class frame) "FdlibmTranslitN$Cbrt")
+     (and (alpha mem loc fixed-sb th s 3)
           (doublep (load-double '(x . 0) mem))
           (doublep (load-double '(t . 0) mem)))))
-  :enable (@cbrt-m0.2-mem sched-m0.2)
+  :enable (alpha @cbrt-m0.2-mem sched-m0.2)
   :use ttt-%0-m0.1)
 
 (defund sched-m0.3 (th)
@@ -655,30 +680,256 @@
           (m5::repeat th 1)
           (get-hi-schedule th)
           (m5::repeat th 1)))
-         
+
 (defrule ttt-%0-m0.3
   (b* (
     (loc (@cbrt-%5-loc (initial-s0 x)))
     (mem (@cbrt-m0.3-mem (initial-s0 x)))
     (s (m5::run (sched-m0.3 th) (initial-s sb th x)))
-    (frame (m5::top-frame th s)))
+    (fixed-sb (m5::modify th sb :call-stack (m5::call-stack th sb) :status 'm5::scheduled)))
     (implies
      (and (doublep x)
           (class-table-assumptions (m5::class-table sb)))
-     (and (@cbrt-local-vars-p loc)
-          (@cbrt-mem-p mem)
-          (pair-p mem (m5::locals frame))
-          (class-table-assumptions (m5::class-table s))
-          (equal (m5::status th s) 'm5::scheduled)
-          (equal (m5::pc frame) 8)
-          (cbrt-compute-program-p (m5::program frame))
-          (equal (m5::cur-class frame) "FdlibmTranslitN$Cbrt")
+     (and (alpha mem loc fixed-sb th s 8)
           (doublep (load-double '(x . 0) mem))
           (i32p (load-i32 '(hx . 0) mem))
           (doublep (load-double '(t . 0) mem)))))
-  :enable (sched-m0.3 poised-to-invoke-get-hi-thm
+  :enable (alpha sched-m0.3 poised-to-invoke-get-hi-thm
     @cbrt-%3-loc @cbrt-%3-val
     @cbrt-%4-loc @cbrt-%4-val
     @cbrt-%5-loc @cbrt-%5-val
     @cbrt-m0.3-mem)
   :use ttt-%0-m0.2)
+
+(defund sched-m0.4 (th)
+  (append (sched-m0.3 th)
+          (m5::repeat th 4)))
+
+(defrule ttt-%0-m0.4
+  (b* (
+    (loc (@cbrt-%7-loc (initial-s0 x)))
+    (mem (@cbrt-m0.4-mem (initial-s0 x)))
+    (s (m5::run (sched-m0.4 th) (initial-s sb th x)))
+    (fixed-sb (m5::modify th sb :call-stack (m5::call-stack th sb) :status 'm5::scheduled)))
+    (implies
+     (and (doublep x)
+          (class-table-assumptions (m5::class-table sb)))
+     (and (alpha mem loc fixed-sb th s 14)
+          (doublep (load-double '(x . 0) mem))
+          (i32p (load-i32 '(hx . 0) mem))
+          (doublep (load-double '(t . 0) mem))
+          (i32p (load-i32 '(sign . 0) mem)))))
+  :enable (alpha sched-m0.4 logand-thm
+    @cbrt-%6-loc @cbrt-%6-val
+    @cbrt-%7-loc @cbrt-%7-val
+    @cbrt-m0.4-mem)
+  :disable m5::bound?
+  :use ttt-%0-m0.3)
+
+(defund sched-m0.5 (th)
+  (append (sched-m0.4 th)
+          (m5::repeat th 4)))
+
+(defrule ttt-%0-m0.5
+  (b* (
+    (loc (@cbrt-%10-loc (initial-s0 x)))
+    (mem (@cbrt-m0.5-mem (initial-s0 x)))
+    (s (m5::run (sched-m0.5 th) (initial-s sb th x)))
+    (fixed-sb (m5::modify th sb :call-stack (m5::call-stack th sb) :status 'm5::scheduled)))
+    (implies
+     (and (doublep x)
+          (class-table-assumptions (m5::class-table sb)))
+     (and (alpha mem loc fixed-sb th s 19)
+          (doublep (load-double '(x . 0) mem))
+          (i32p (load-i32 '(hx . 0) mem))
+          (doublep (load-double '(t . 0) mem))
+          (i32p (load-i32 '(sign . 0) mem)))))
+  :enable (alpha sched-m0.5 logxor-thm
+    @cbrt-%8-loc @cbrt-%8-val
+    @cbrt-%9-loc @cbrt-%9-val
+    @cbrt-%10-loc @cbrt-%10-val
+    @cbrt-m0.5-mem)
+  :disable logxor
+  :use ttt-%0-m0.4)
+
+(defund sched-succ0 (th)
+  (append (sched-m0.5 th)
+          (m5::repeat th 3)))
+
+(defrule ttt-%0-succ0
+  (b* (
+    (loc (@cbrt-%12-loc (initial-s0 x)))
+    (mem (@cbrt-m0.5-mem (initial-s0 x)))
+    (lab (@cbrt-succ0-lab (initial-s0 x)))
+    (s (m5::run (sched-succ0 th) (initial-s sb th x)))
+    (fixed-sb (m5::modify th sb :call-stack (m5::call-stack th sb) :status 'm5::scheduled)))
+    (implies
+     (and (doublep x)
+          (class-table-assumptions (m5::class-table sb)))
+     (and (alpha mem loc fixed-sb th s (case lab (%13 25) (%17 29)))
+          (member lab '(%13 %17))
+          (doublep (load-double '(x . 0) mem))
+          (i32p (load-i32 '(hx . 0) mem))
+          (doublep (load-double '(t . 0) mem))
+          (i32p (load-i32 '(sign . 0) mem)))))
+  :enable (alpha sched-succ0 icmp-sge-i32
+    @cbrt-%11-loc @cbrt-%11-val
+    @cbrt-%12-loc @cbrt-%12-val
+    @cbrt-succ0-lab)
+  :disable m5::bound?
+  :use ttt-%0-m0.5)
+
+;----------------------------
+
+(defund sched-m13.1 (th)
+  (m5::repeat th 3))
+
+(defrule ttt-%13-m13.1
+  (b* (
+    (s13 (list mem13 loc13 '%0))
+    (loc (@cbrt-%16-loc s13))
+    (mem (@cbrt-m13.1-mem s13))
+    (s (m5::run (sched-m13.1 th) s-old)))
+    (implies
+     (and (alpha mem13 loc13 sb th s-old 25)
+          (doublep (load-double '(x . 0) mem13)))
+     (and (alpha mem loc sb th s 28)
+          (doublep (load-double '(ret . 0) mem))
+          (equal (m5::top2 (m5::stack (m5::top-frame th s)))
+                 (load-double '(ret . 0) mem)))))
+  :enable (alpha sched-m13.1 fpadd-thm
+    @cbrt-%13-mem @cbrt-%13-loc
+    @cbrt-%14-loc @cbrt-%14-val
+    @cbrt-%15-loc @cbrt-%15-val
+    @cbrt-%16-loc @cbrt-%16-val
+    @cbrt-m13.1-mem)
+  :disable m5::fpadd)
+
+(defund sched-succ13 (th)
+  (append (sched-m13.1 th)
+          (m5::repeat th 1)))
+
+(defrule ttt-%13-succ13
+  (b* (
+    (s13 (list mem13 loc13 '%0))
+    (loc (@cbrt-%16-loc s13))
+    (mem (@cbrt-m13.1-mem s13))
+    (lab (@cbrt-succ13-lab s13))
+    (s (m5::run (sched-succ13 th) s-old)))
+    (implies
+     (and (alpha mem13 loc13 sb th s-old 25)
+          (doublep (load-double '(x . 0) mem13)))
+     (and (equal lab '%101)
+          (equal (g '%1 loc) '(ret . 0))
+          (doublep (load-double '(ret . 0) mem))
+          (equal s (ret-double th sb (load-double '(ret . 0) mem))))))
+  :enable (sched-succ13 ret-thm-when-alpha
+                 @cbrt-succ13-lab)
+  :use ttt-%13-m13.1)
+
+;--------------------------------
+
+(defund sched-succ17 (th)
+  (append (m5::repeat th 2)
+          (get-lo-schedule th)
+          (m5::repeat th 2)))
+
+(defrule ttt-%17-succ17
+  (b* (
+    (s17 (list mem17 loc17 '%0))
+    (loc (@cbrt-%22-loc s17))
+    (mem (@cbrt-%17-mem s17))
+    (lab (@cbrt-succ17-lab s17))
+    (s (m5::run (sched-succ17 th) s-old)))
+    (implies
+     (and (alpha mem17 loc17 sb th s-old 29)
+          (i32p (load-i32 '(hx . 0) mem17))
+          (doublep (load-double '(t . 0) mem17))
+          (i32p (load-i32 '(sign . 0) mem17))
+          (doublep (load-double '(x . 0) mem17)))
+     (and (alpha mem loc sb th s (case lab (%23 38) (%25 40)))
+          (member lab '(%23 %25))
+          (doublep (load-double '(x . 0) mem))
+          (i32p (load-i32 '(hx . 0) mem))
+          (doublep (load-double '(t . 0) mem))
+          (i32p (load-i32 '(sign . 0) mem)))))
+  :enable (alpha sched-succ17 poised-to-invoke-get-lo-thm logior-thm icmp-eq-i32
+    @cbrt-%17-loc @cbrt-%17-mem
+    @cbrt-%18-loc @cbrt-%18-val
+    @cbrt-%19-loc @cbrt-%19-val
+    @cbrt-%20-loc @cbrt-%20-val
+    @cbrt-%21-loc @cbrt-%21-val
+    @cbrt-%22-loc @cbrt-%22-val
+    @cbrt-succ17-lab)
+  :disable logior)
+
+;--------------------------------
+
+(defund sched-m23.1 (th)
+  (m5::repeat th 1))
+
+(defrule ttt-%23-m23.1
+  (b* (
+    (s23 (list mem23 loc23 '%0))
+    (loc (@cbrt-%24-loc s23))
+    (mem (@cbrt-m23.1-mem s23))
+    (s (m5::run (sched-m23.1 th) s-old)))
+    (implies
+     (and (alpha mem23 loc23 sb th s-old 38)
+          (doublep (load-double '(x . 0) mem23)))
+     (and (alpha mem loc sb th s 39)
+          (doublep (load-double '(ret . 0) mem))
+          (equal (m5::top2 (m5::stack (m5::top-frame th s)))
+                 (load-double '(ret . 0) mem)))))
+  :enable (alpha sched-m23.1
+    @cbrt-%23-mem @cbrt-%23-loc
+    @cbrt-%24-loc @cbrt-%24-val
+    @cbrt-m23.1-mem))
+
+(defund sched-succ23 (th)
+  (append (sched-m23.1 th)
+          (m5::repeat th 1)))
+
+(defrule ttt-%23-succ23
+  (b* (
+    (s23 (list mem23 loc23 '%0))
+    (loc (@cbrt-%24-loc s23))
+    (mem (@cbrt-m23.1-mem s23))
+    (lab (@cbrt-succ23-lab s23))
+    (s (m5::run (sched-succ23 th) s-old)))
+    (implies
+     (and (alpha mem23 loc23 sb th s-old 38)
+          (doublep (load-double '(x . 0) mem23)))
+     (and (equal lab '%101)
+          (equal (g '%1 loc) '(ret . 0))
+          (doublep (load-double '(ret . 0) mem))
+          (equal s (ret-double th sb (load-double '(ret . 0) mem))))))
+  :enable (sched-succ23 ret-thm-when-alpha
+    @cbrt-succ23-lab)
+  :use ttt-%23-m23.1)
+
+;------------------------------
+
+;--------------------------------
+
+(defund sched-succ101 (th)
+  (m5::repeat th 0))
+
+(defrule ttt-%101-succ101
+  (b* (
+    (s101 (list mem101 loc101 pred))
+    (mem (@cbrt-%101-mem s101))
+    (loc (@cbrt-%102-loc s101))
+    (lab (@cbrt-succ101-lab s101))
+    (s (m5::run (sched-succ101 th) s-old)))
+    (implies
+     (and (equal (g '%1 loc) '(ret . 0))
+          (doublep (load-double '(ret . 0) mem))
+          (equal s (ret-double th sb (load-double '(ret . 0) mem))))
+     (and (equal lab 'ret)
+          (doublep (g '%102 loc))
+          (equal s (ret-double th sb (g '%102 loc))))))
+  :enable (sched-succ101
+    @cbrt-%101-loc @cbrt-%101-mem
+    @cbrt-%102-loc @cbrt-%102-val
+    @cbrt-succ101-lab))
