llvm2acl2/acl2/llvm-rec.lisp
@@ -21,8 +21,13 @@
        (<= (- (expt 2 31)) x)
        (< x (expt 2 31))))
 
+(defund i64p (x)
+  (and (integerp x)
+       (<= (- (expt 2 63)) x)
+       (< x (expt 2 63))))
+
 (defund get-lo-i32 (x)
-  (m5::uint-fix x))
+  (and (i32p x) (m5::uint-fix x)))
 
 (defund make-i32 (w0)
   (and (wordp w0) (m5::int-fix w0)))
@@ -31,19 +36,22 @@
   (rtl::encodingp x (rtl::dp)))
 
 (defund get-lo-double (d)
-  (m5::uint-fix d))
+  (and (doublep d) (m5::uint-fix d)))
 
 (defund get-hi-double (d)
-  (m5::uint-fix (m5::shr (ifix d) 32)))
+  (and (doublep d) (m5::uint-fix (m5::shr (ifix d) 32))))
 
 (defund make-double (w1 w0)
   (and (wordp w1) (wordp w0) (rtl::cat w1 32 w0 32)))
 
-(defund alloca-double-1 (var mem)
-  (mv (cons var 0) (s var '(nil nil) mem)))
+(defund alloca-double (var n mem)
+  (s var (make-list (* 2 n)) mem))
 
-(defund alloca-i32-1 (var mem)
-  (mv (cons var 0) (s var '(nil) mem)))
+(defund alloca-i32 (var n mem)
+  (s var (make-list n) mem))
+
+(defund alloca-pointer (var mem)
+  (s var '(nil) mem))
 
 (defund store-double (d a mem)
   (let* ((var (car a))
@@ -62,6 +70,14 @@
          (new (update-nth ofs w0 old)))
     (s var new mem)))
 
+(defund store-pointer (p a mem)
+  (let* ((var (car a))
+         (ofs (cdr a))
+         (old (g var mem))
+         (w0 (and (addressp p) p))
+         (new (update-nth ofs w0 old)))
+    (s var new mem)))
+
 (defund load-double (a mem)
   (let* ((var (car a))
          (ofs (cdr a))
@@ -77,13 +93,37 @@
          (w0 (nth ofs val)))
     (and (wordp w0) (make-i32 w0))))
 
+(defund load-pointer (a mem)
+  (let* ((var (car a))
+         (ofs (cdr a))
+         (val (g var mem))
+         (w0 (nth ofs val)))
+    (and (addressp w0) w0)))
+
+(defund getelementptr-double (a i)
+  (and (addressp a)
+       (i64p i)
+       (cons (car a) (+ (cdr a) (* 2 i)))))
+
 (defund getelementptr-i32 (a i)
   (and (addressp a)
-       (i32p i)
+       (i64p i)
        (cons (car a) (+ (cdr a) i))))
 
 (defund bitcast-double*-to-i32* (a)
   (and (addressp a) a))
+
+(defund sext-i32-to-i64 (x)
+  (and (i32p x) x))
+
+(defund zext-i32-to-i64 (x)
+  (and (i32p x) (m5::ulong-fix x)))
+
+(defund fptosi-double-to-i32 (x)
+  (and (doublep x) (m5::fp2int x (rtl::dp) 32)))
+
+(defund sitofp-i32-to-double (x)
+  (and (i32p x) (m5::int2fp x (rtl::dp))))
 
 (defund fadd-double (x y)
   (and (doublep x) (doublep y) (m5::fpadd x y (rtl::dp))))
@@ -97,11 +137,32 @@
 (defund fdiv-double (x y)
   (and (doublep x) (doublep y) (m5::fpdiv x y (rtl::dp))))
 
+(defund fcmp-oeq-double (x y)
+  (and (doublep x) (doublep y) (if (= (m5::fpcmp x y (rtl::dp) -1) 0) -1 0)))
+
+(defund fcmp-oge-double (x y)
+  (and (doublep x) (doublep y) (if (>= (m5::fpcmp x y (rtl::dp) -1) 0) -1 0)))
+
+(defund fcmp-ogt-double (x y)
+  (and (doublep x) (doublep y) (if (equal (m5::fpcmp x y (rtl::dp) -1) +1) -1 0)))
+
+(defund fcmp-ole-double (x y)
+  (and (doublep x) (doublep y) (if (<= (m5::fpcmp x y (rtl::dp) +1) 0) -1 0)))
+
+(defund fcmp-olt-double (x y)
+  (and (doublep x) (doublep y) (if (equal (m5::fpcmp x y (rtl::dp) +1) -1) -1 0)))
+
 (defund add-i32 (x y)
   (and (i32p x) (i32p y) (m5::int-fix (+ x y))))
 
+(defund sub-i32 (x y)
+  (and (i32p x) (i32p y) (m5::int-fix (- x y))))
+
+(defund mul-i32 (x y)
+  (and (i32p x) (i32p y) (m5::int-fix (* x y))))
+
 (defund sdiv-i32 (x y)
-  (and (i32p x) (i32p y) (not (= y 0)) (m5::int-fix (/ x y))))
+  (and (i32p x) (i32p y) (not (= y 0)) (m5::int-fix (truncate x y))))
 
 (defund and-i32 (x y)
   (and (i32p x) (i32p y) (logand x y)))
@@ -112,12 +173,58 @@
 (defund xor-i32 (x y)
   (and (i32p x) (i32p y) (logxor x y)))
 
+(defund shl-i32 (x y)
+  (and (i32p x) (i32p y) (m5::int-fix (m5::shl x (m5::5-bit-fix y)))))
+
+(defund lshr-i32 (x y)
+  (and (i32p x) (i32p y) (m5::int-fix (m5::shr (m5::uint-fix x) (m5::5-bit-fix y)))))
+
+(defund ashr-i32 (x y)
+  (and (i32p x) (i32p y) (m5::int-fix (m5::shr x (m5::5-bit-fix y)))))
+
 (defund icmp-eq-i32 (x y)
   (and (i32p x) (i32p y) (if (= x y) -1 0)))
+
+(defund icmp-ne-i32 (x y)
+  (and (i32p x) (i32p y) (if (not (= x y)) -1 0)))
 
 (defund icmp-slt-i32 (x y)
   (and (i32p x) (i32p y) (if (< x y) -1 0)))
 
+(defund icmp-sle-i32 (x y)
+  (and (i32p x) (i32p y) (if (<= x y) -1 0)))
+
+(defund icmp-sgt-i32 (x y)
+  (and (i32p x) (i32p y) (if (> x y) -1 0)))
+
 (defund icmp-sge-i32 (x y)
   (and (i32p x) (i32p y) (if (>= x y) -1 0)))
 
+(defund icmp-ult-i32 (x y)
+  (and (i32p x) (i32p y) (if (< (m5::uint-fix x) (m5::uint-fix y)) -1 0)))
+
+(defund icmp-ule-i32 (x y)
+  (and (i32p x) (i32p y) (if (<= (m5::uint-fix x) (m5::uint-fix y)) -1 0)))
+
+(defund icmp-ugt-i32 (x y)
+  (and (i32p x) (i32p y) (if (> (m5::uint-fix x) (m5::uint-fix y)) -1 0)))
+
+(defund icmp-uge-i32 (x y)
+  (and (i32p x) (i32p y) (if (>= (m5::uint-fix x) (m5::uint-fix y)) -1 0)))
+
+(defund select-double (x y z)
+  (and (i1p x) (doublep y) (doublep z) (if (not (= x 0)) y z)))
+
+;--------
+
+(defund get-lo (d)
+  (make-i32 (get-lo-double d)))
+
+(defund get-hi (d)
+  (make-i32 (get-hi-double d)))
+
+(defund set-lo (d lo)
+  (make-double (get-hi-double d) (get-lo-i32 lo)))
+
+(defund set-hi (d hi)
+  (make-double (get-lo-i32 hi) (get-lo-double d)))
