llvm2acl2/acl2/llvm-rec-lemmas.lisp
@@ -116,6 +116,91 @@
 
 ;----------
 
+(local
+ (defruled uint-fix-as-bits
+   (equal (m5::uint-fix x)
+          (rtl::bits (ifix x) 31 0))
+   :enable rtl::bits-mod
+   :disable mod))
+
+(local
+ (defruled double-fix-as-bits
+   (equal (m5::double-fix x)
+          (rtl::bits (ifix x) 63 0))
+   :enable rtl::bits-mod
+   :disable mod))
+
+(defrule make-i32-get-lo-32
+  (implies (i32p x)
+           (equal (make-i32 (get-lo-i32 x))
+                  x))
+  :enable (get-lo-i32 make-i32 i32p wordp))
+
+(defrule get-lo-i32-make-i32
+  (implies (wordp w0)
+           (equal (get-lo-i32 (make-i32 w0))
+                  w0))
+  :enable (get-lo-i32 make-i32 wordp i32p))
+
+(local
+ (defruled get-lo-double-as-bits
+   (equal (get-lo-double d)
+          (and (doublep d) (rtl::bits (ifix d) 31 0)))
+   :enable (get-lo-double uint-fix-as-bits)
+   :disable m5::uint-fix))
+
+(local
+ (with-arith5-help
+  (defruled bits-shr
+    (implies (and (integerp k)
+                  (integerp i)
+                  (natp j))
+             (equal (rtl::bits (m5::shr x k) i j)
+                    (rtl::bits x (+ i k) (+ j k))))
+    :enable rtl::fl
+    :disable floor
+    :use rtl::bits-shift-down-1)))
+
+(local
+ (defruled get-hi-double-as-bits
+   (equal (get-hi-double d)
+          (and (doublep d) (rtl::bits (ifix d) 63 32)))
+   :enable (get-hi-double uint-fix-as-bits bits-shr)
+   :disable (m5::uint-fix m5::shr)))
+
+(defrule make-double-get-hi-get-lo
+  (implies (doublep d)
+           (equal (make-double (get-hi-double d) (get-lo-double d))
+                  d))
+  :enable (make-double doublep rtl::encodingp rtl::dp)
+  :disable (m5::double-fix m5::ulong-fix m5::shr)
+  :cases ((and (wordp (get-hi-double d)) (wordp (get-lo-double d))))
+  :hints
+  (("subgoal 2" :in-theory (enable wordp get-lo-double get-hi-double))
+   ("subgoal 1" :in-theory (enable get-hi-double-as-bits get-lo-double-as-bits))))
+
+(defrule make-double-type
+  (implies (and (wordp w0)
+                (wordp w1))
+           (doublep (make-double w1 w0)))
+  :enable (doublep make-double rtl::encodingp rtl::dp))
+
+(defrule get-hi-double-make-double
+  (implies (and (wordp w1) (wordp w0))
+           (equal (get-hi-double (make-double w1 w0))
+                  w1))
+  :enable (make-double get-hi-double-as-bits wordp rtl::bits rtl::fl)
+  :use make-double-type)
+
+(defrule get-lo-double-make-double
+  (implies (and (wordp w1) (wordp w0))
+           (equal (get-lo-double (make-double w1 w0))
+                  w0))
+  :enable (make-double get-lo-double-as-bits wordp rtl::bits rtl::fl)
+  :use make-double-type)
+
+;----------
+
 (defrule get-lo-i32-type
   (implies (i32p i)
            (wordp (get-lo-i32 i)))
@@ -148,7 +233,7 @@
            (doublep (load-double (cons var ofs) mem)))
   :enable (addressp load-double))
 
-(defrule store-double-type
+(defruled store-double-type
   (implies (doublep d)
            (equal (store-double d (cons var ofs) mem)
                   (s
@@ -163,12 +248,11 @@
                    mem)))
   :enable store-double)
 
-
 (defrule getelementptr-i32-type
   (implies (and (addressp a)
-                (i32p i))
+                (i64p i))
            (addressp (getelementptr-i32 a i)))
-  :enable (addressp i32p getelementptr-i32))
+  :enable (addressp i64p getelementptr-i32))
 
 (defrule bitcast-double*-to-i32*-type
   (implies (addressp a)
@@ -210,6 +294,13 @@
   :enable add-i32
   :disable m5::int-fix)
 
+(defrule sub-i32-type
+  (implies (and (i32p x)
+                (i32p y))
+           (i32p (sub-i32 x y)))
+  :enable sub-i32
+  :disable m5::int-fix)
+
 (defrule sdiv-i32-type
   (implies (and (i32p x)
                 (i32p y)
@@ -236,11 +327,38 @@
            (i32p (xor-i32 x y)))
   :enable (i32p-as-signed-byte-p xor-i32))
 
+(defrule shl-i32-type
+  (implies (and (i32p x)
+                (i32p y))
+           (i32p (shl-i32 x y)))
+  :enable shl-i32
+  :disable m5::int-fix)
+
+(defrule lshr-i32-type
+  (implies (and (i32p x)
+                (i32p y))
+           (i32p (lshr-i32 x y)))
+  :enable lshr-i32
+  :disable m5::int-fix)
+
+(defrule ashr-i32-type
+  (implies (and (i32p x)
+                (i32p y))
+           (i32p (ashr-i32 x y)))
+  :enable ashr-i32
+  :disable m5::int-fix)
+
 (defrule icmp-eq-i32-type
   (implies (and (i32p x)
                 (i32p y))
            (i1p (icmp-eq-i32 x y)))
   :enable icmp-eq-i32)
+
+(defrule icmp-ne-i32-type
+  (implies (and (i32p x)
+                (i32p y))
+           (i1p (icmp-ne-i32 x y)))
+  :enable icmp-ne-i32)
 
 (defrule icmp-slt-i32-type
   (implies (and (i32p x)
@@ -248,8 +366,74 @@
            (i1p (icmp-slt-i32 x y)))
   :enable icmp-slt-i32)
 
+(defrule icmp-sle-i32-type
+  (implies (and (i32p x)
+                (i32p y))
+           (i1p (icmp-sle-i32 x y)))
+  :enable icmp-sle-i32)
+
+(defrule icmp-sgt-i32-type
+  (implies (and (i32p x)
+                (i32p y))
+           (i1p (icmp-sgt-i32 x y)))
+  :enable icmp-sgt-i32)
+
 (defrule icmp-sge-i32-type
   (implies (and (i32p x)
                 (i32p y))
            (i1p (icmp-sge-i32 x y)))
   :enable icmp-sge-i32)
+
+(defrule icmp-ult-i32-type
+  (implies (and (i32p x)
+                (i32p y))
+           (i1p (icmp-ult-i32 x y)))
+  :enable icmp-ult-i32)
+
+(defrule icmp-ule-i32-type
+  (implies (and (i32p x)
+                (i32p y))
+           (i1p (icmp-ule-i32 x y)))
+  :enable icmp-ule-i32)
+
+(defrule icmp-ugt-i32-type
+  (implies (and (i32p x)
+                (i32p y))
+           (i1p (icmp-ugt-i32 x y)))
+  :enable icmp-ugt-i32)
+
+(defrule icmp-uge-i32-type
+  (implies (and (i32p x)
+                (i32p y))
+           (i1p (icmp-uge-i32 x y)))
+  :enable icmp-uge-i32)
+
+(defruled i1p=-1
+  (implies (i1p x)
+           (equal (equal x -1)
+                  (not (equal x 0))))
+  :enable i1p)
+
+;--------
+
+(defrule get-lo-type
+  (implies (doublep d)
+           (i32p (get-lo d)))
+  :enable get-lo)
+
+(defrule get-hi-type
+  (implies (doublep d)
+           (i32p (get-hi d)))
+  :enable get-hi)
+
+(defrule set-lo-type
+  (implies (and (doublep d)
+                (i32p lo))
+           (doublep (set-lo d lo)))
+  :enable set-lo)
+
+(defrule set-hi-type
+  (implies (and (doublep d)
+                (i32p hi))
+           (doublep (set-hi d hi)))
+  :enable set-hi)
